Unfinished. There are things that should be fix from the foundations at the tree level.

Verification for Buddy Memory Allocation/Memory_Allocation_Model.thy
@@ -91,6 +91,30 @@ fun get_level_node' :: "'a tree \<Rightarrow> 'a tree \<Rightarrow> nat \<Righta
 definition get_level_node :: "'a tree \<Rightarrow> 'a tree \<Rightarrow> nat"
   where "get_level_node B b \<equiv> get_level_node' B b 0"
 
+fun is_subtree ::"'a tree \<Rightarrow> 'a tree \<Rightarrow> bool"
+  where "is_subtree (Leaf x) n = (if (n=(Leaf x)) then True else False)" 
+  | "is_subtree (Node n1 n2 n3 n4) n = (if (n= (Node n1 n2 n3 n4)) then True 
+                                        else 
+                                         is_subtree n1 n \<or> is_subtree n2 n \<or> 
+                                         is_subtree n3 n \<or> is_subtree n4 n)"
+
+lemma is_subtree_subset:"is_subtree N n \<Longrightarrow> set n \<subseteq> set N"
+proof(induct N)
+  case (Leaf x)
+  then show ?case
+    by (metis is_subtree.simps(1) order_refl) 
+  next
+    case (Node N1 N2 N3 N4)
+    then show ?case
+      by (metis is_subtree.simps(2) set_mp subsetI sup.coboundedI2 
+          tree.set_intros(2) tree.set_intros(3) tree.set_intros(4) tree.simps(16)) 
+  qed
+
+lemma "N\<noteq>n \<Longrightarrow> is_subtree N n \<Longrightarrow> get_level_node N n > 0"
+
+
+lemma "get_level_node B b = 0 \<Longrightarrow> (B = b) \<or> (\<exists>x. B = Leaf x)"
+
 lemma level_node_notbelong:
   "leaf b \<Longrightarrow>
   L b \<notin> set B \<Longrightarrow>
@@ -173,6 +197,11 @@ next
   then show ?case using l_node' l_node by auto
 qed
 
+definition set_state_type :: "Block \<Rightarrow> block_state_type \<Rightarrow> Block"
+  where "set_state_type bl t \<equiv> (let b = (L bl) in Leaf (t, snd b))"
+
+
+
 subsection \<open>def of function_call\<close>
 (*------------------------------------------------------------------------------------------------*)
 inductive id_not_in_mem :: "Block \<Rightarrow> ID \<Rightarrow> bool"
@@ -184,6 +213,8 @@ inductive_cases id_not_in_mem_node:
 
 definition id_not_in_set_mem::"Block set \<Rightarrow> ID \<Rightarrow> bool"
   where "id_not_in_set_mem bs v \<equiv> \<forall>b \<in> bs. id_not_in_mem b v"
+
+
 
 lemma finite_ids_set:"finite (snd ` set b)"
 proof (induct b)
@@ -249,6 +280,554 @@ next
   then show ?case using not_in_mem_not_in_set unfolding id_not_in_set_mem_def
     by (meson UN_iff)    
 qed
+
+fun replace_leaf :: "Block \<Rightarrow> Block \<Rightarrow> Block \<Rightarrow> Block"
+  where "replace_leaf (Leaf x) y st = (if (x = (L y)) then st else (Leaf x))" |
+        "replace_leaf (Node n1 n2 n3 n4) y st = Node (replace_leaf n1 y st)
+                                                     (replace_leaf n2 y st)
+                                                     (replace_leaf n3 y st)
+                                                     (replace_leaf n4 y st)"
+
+lemma "get_level_node t (Leaf x) \<noteq> 0 \<Longrightarrow> set (replace_leaf t (Leaf x) nr) = 
+        (((set t) - (set (Leaf x))) \<union> (set nr))"
+  sorry
+
+lemma "t\<noteq>(Leaf x) \<Longrightarrow> get_level_node t (Leaf x) = 0 \<Longrightarrow> replace_leaf t (Leaf x) nr = t"
+proof(induct t)
+  case (Leaf x)
+  then show ?case
+    by simp 
+next
+  case (Node t1 t2 t3 t4)
+  then show ?case sorry
+qed
+
+lemma no_replace:
+  "L b \<notin> set blo \<Longrightarrow>
+  b' = set_state_type b t \<Longrightarrow>
+  tree_map (\<lambda>b1. if b1 = L b then L b' else b1) blo = blo"
+  by (smt tree.map_cong0 tree.map_ident)
+
+lemma no_replace_leaf:
+  "(L b) \<notin> set B \<Longrightarrow>
+  replace_leaf B b subbtr = B"
+  apply(induct B)
+  by auto
+
+lemma replace_leaf_belong:
+  "(L b) \<in> set B \<Longrightarrow>
+  (L l) \<in> set subbtr \<Longrightarrow>
+  (L l) \<in> set (replace_leaf B b subbtr)"
+  apply(induct B)
+  by auto
+
+lemma replace_subbtr_belong:
+  "(L b) \<in> set B \<Longrightarrow>
+  tree.set subbtr \<subseteq> tree.set (replace_leaf B b subbtr)"
+  apply(induct B)
+  by auto
+
+subsection \<open>def and proof of inv_different_ids\<close>
+
+definition id_set :: "Block \<Rightarrow> ID set"
+  where "id_set b \<equiv> snd ` (set b)"
+
+lemma id_set_node:
+  "id_set (Node b1 b2 b3 b4) = id_set b1 \<union> id_set b2 \<union> id_set b3 \<union> id_set b4"
+  unfolding id_set_def by auto
+
+lemma id_set_notempty: "id_set B \<noteq> {}"
+  apply(induct B)
+  unfolding id_set_def apply auto[1]
+  using id_set_node unfolding id_set_def by auto
+
+inductive diff_ids:: "Block \<Rightarrow> bool"
+  where diff1: "diff_ids (Leaf a)" |
+        diff2: "(id_set b1) \<inter> (id_set b2) = {} \<and> (id_set b1) \<inter> (id_set b3) = {} \<and> (id_set b1) \<inter> (id_set b4) = {} \<and>
+                (id_set b2) \<inter> (id_set b3) = {} \<and> (id_set b2) \<inter> (id_set b4) = {} \<and>
+                (id_set b3) \<inter> (id_set b4) = {} \<and>
+                diff_ids b1 \<and> diff_ids b2 \<and> diff_ids b3 \<and> diff_ids b4 \<Longrightarrow> diff_ids (Node b1 b2 b3 b4)"
+
+inductive_cases diff_ids_leaf_node:
+  "diff_ids (Leaf a)"
+  "diff_ids (Node ll lr rl rr)"
+
+
+lemma diff_leaf1:
+  "diff_ids (Node b1 b2 b3 b4) \<Longrightarrow>
+  (L l) \<in> set b1 \<Longrightarrow>
+  (L l) \<notin> set b2 \<and> (L l) \<notin> set b3 \<and> (L l) \<notin> set b4"
+proof-
+  assume a0: "diff_ids (Node b1 b2 b3 b4)"
+     and a1: "(L l) \<in> set b1"
+  have diff_ab: "(id_set b1) \<inter> (id_set b2) = {}"
+    using a0 diff_ids_leaf_node(2) by blast
+  have diff_ac: "(id_set b1) \<inter> (id_set b3) = {}"
+    using a0 diff_ids_leaf_node(2) by blast
+  have diff_ad: "(id_set b1) \<inter> (id_set b4) = {}"
+    using a0 diff_ids_leaf_node(2) by blast
+  have l_id: "snd (L l) \<in> id_set b1"
+    unfolding id_set_def using a1
+    by (simp add: tree.set_map) 
+  have n1: "snd (L l) \<notin> id_set b2"
+    using diff_ab l_id by auto
+  have n2: "snd (L l) \<notin> id_set b3"
+    using diff_ac l_id by auto
+  have n3: "snd (L l) \<notin> id_set b4"
+    using diff_ad l_id by auto
+  show ?thesis using n1 n2 n3
+    using id_set_def tree.set_map by fastforce 
+qed
+
+lemma diff_leaf2:
+  "diff_ids (Node b1 b2 b3 b4) \<Longrightarrow>
+  (L l) \<in> set b2 \<Longrightarrow>
+  (L l) \<notin> set b1 \<and> (L l) \<notin> set b3 \<and> (L l) \<notin> set b4"
+proof-
+  assume a0: "diff_ids (Node b1 b2 b3 b4)"
+     and a1: "(L l) \<in> set b2"
+  have diff_ab: "(id_set b2) \<inter> (id_set b1) = {}"
+    using a0 diff_ids_leaf_node(2) by blast
+  have diff_bc: "(id_set b2) \<inter> (id_set b3) = {}"
+    using a0 diff_ids_leaf_node(2) by blast
+  have diff_bd: "(id_set b2) \<inter> (id_set b4) = {}"
+    using a0 diff_ids_leaf_node(2) by blast
+  have l_id: "snd (L l) \<in> id_set b2"
+    unfolding id_set_def using a1
+    by (simp add: tree.set_map) 
+  have n1: "snd (L l) \<notin> id_set b1"
+    using diff_ab l_id by auto
+  have n2: "snd (L l) \<notin> id_set b3"
+    using diff_bc l_id by auto
+  have n3: "snd (L l) \<notin> id_set b4"
+    using diff_bd l_id by auto
+  show ?thesis using n1 n2 n3
+    using id_set_def tree.set_map by fastforce 
+qed
+
+lemma diff_leaf3:
+  "diff_ids (Node b1 b2 b3 b4) \<Longrightarrow>
+  (L l) \<in> set b3 \<Longrightarrow>
+  (L l) \<notin> set b1 \<and> (L l) \<notin> set b2 \<and> (L l) \<notin> set b4"
+proof-
+  assume a0: "diff_ids (Node b1 b2 b3 b4)"
+     and a1: "(L l) \<in> set b3"
+  have diff_ac: "(id_set b3) \<inter> (id_set b1) = {}"
+    using a0 diff_ids_leaf_node(2) by blast
+  have diff_bc: "(id_set b3) \<inter> (id_set b2) = {}"
+    using a0 diff_ids_leaf_node(2) by blast
+  have diff_cd: "(id_set b3) \<inter> (id_set b4) = {}"
+    using a0 diff_ids_leaf_node(2) by blast
+  have l_id: "snd (L l) \<in> id_set b3"
+    unfolding id_set_def using a1
+    by (simp add: tree.set_map) 
+  have n1: "snd (L l) \<notin> id_set b1"
+    using diff_ac l_id by auto
+  have n2: "snd (L l) \<notin> id_set b2"
+    using diff_bc l_id by auto
+  have n3: "snd (L l) \<notin> id_set b4"
+    using diff_cd l_id by auto
+  show ?thesis using n1 n2 n3
+    using id_set_def tree.set_map by fastforce 
+qed
+
+lemma diff_leaf4:
+  "diff_ids (Node b1 b2 b3 b4) \<Longrightarrow>
+  (L l) \<in> set b4 \<Longrightarrow>
+  (L l) \<notin> set b1 \<and> (L l) \<notin> set b2 \<and> (L l) \<notin> set b3"
+proof-
+  assume a0: "diff_ids (Node b1 b2 b3 b4)"
+     and a1: "(L l) \<in> set b4"
+  have diff_ad: "(id_set b4) \<inter> (id_set b1) = {}"
+    using a0 diff_ids_leaf_node(2) by blast
+  have diff_bd: "(id_set b4) \<inter> (id_set b2) = {}"
+    using a0 diff_ids_leaf_node(2) by blast
+  have diff_cd: "(id_set b4) \<inter> (id_set b3) = {}"
+    using a0 diff_ids_leaf_node(2) by blast
+  have l_id: "snd (L l) \<in> id_set b4"
+    unfolding id_set_def using a1
+    by (simp add: tree.set_map) 
+  have n1: "snd (L l) \<notin> id_set b1"
+    using diff_ad l_id by auto
+  have n2: "snd (L l) \<notin> id_set b2"
+    using diff_bd l_id by auto
+  have n3: "snd (L l) \<notin> id_set b3"
+    using diff_cd l_id by auto
+  show ?thesis using n1 n2 n3
+    using id_set_def tree.set_map by fastforce 
+qed 
+
+lemma diff_node1:
+  "diff_ids (Node b1 b2 b3 b4) \<Longrightarrow>
+  tree.set subbtr \<subseteq> tree.set b1 \<Longrightarrow>
+  \<not> tree.set subbtr \<subseteq> tree.set b2 \<and> \<not> tree.set subbtr \<subseteq> tree.set b3 \<and> \<not> tree.set subbtr \<subseteq> tree.set b4"
+proof-
+  assume a0: "diff_ids (Node b1 b2 b3 b4)"
+     and a1: "tree.set subbtr \<subseteq> tree.set b1"
+  have diff_ab: "(id_set b1) \<inter> (id_set b2) = {}"
+    using a0 diff_ids_leaf_node(2) by blast
+  have diff_ac: "(id_set b1) \<inter> (id_set b3) = {}"
+    using a0 diff_ids_leaf_node(2) by blast
+  have diff_ad: "(id_set b1) \<inter> (id_set b4) = {}"
+    using a0 diff_ids_leaf_node(2) by blast
+  have subbtr_id: "id_set subbtr \<subseteq> id_set b1"
+    unfolding id_set_def using a1
+    by (metis subset_image_iff tree.set_map)
+  have n1: "\<not> id_set subbtr \<subseteq> id_set b2"
+    using diff_ab subbtr_id id_set_notempty by fastforce
+  have n2: "\<not> id_set subbtr \<subseteq> id_set b3"
+    using diff_ac subbtr_id id_set_notempty by fastforce
+  have n3: "\<not> id_set subbtr \<subseteq> id_set b4"
+    using diff_ad subbtr_id id_set_notempty by fastforce
+  show ?thesis using n1 n2 n3 unfolding id_set_def
+    by (metis subset_image_iff tree.set_map)
+qed
+
+lemma diff_node2:
+  "diff_ids (Node b1 b2 b3 b4) \<Longrightarrow>
+  tree.set subbtr \<subseteq> tree.set b2 \<Longrightarrow>
+  \<not> tree.set subbtr \<subseteq> tree.set b1 \<and> \<not> tree.set subbtr \<subseteq> tree.set b3 \<and> \<not> tree.set subbtr \<subseteq> tree.set b4"
+proof-
+  assume a0: "diff_ids (Node b1 b2 b3 b4)"
+     and a1: "tree.set subbtr \<subseteq> tree.set b2"
+  have diff_ab: "(id_set b2) \<inter> (id_set b1) = {}"
+    using a0 diff_ids_leaf_node(2) by blast
+  have diff_bc: "(id_set b2) \<inter> (id_set b3) = {}"
+    using a0 diff_ids_leaf_node(2) by blast
+  have diff_bd: "(id_set b2) \<inter> (id_set b4) = {}"
+    using a0 diff_ids_leaf_node(2) by blast
+  have subbtr_id: "id_set subbtr \<subseteq> id_set b2"
+    unfolding id_set_def using a1
+    by (metis subset_image_iff tree.set_map)
+  have n1: "\<not> id_set subbtr \<subseteq> id_set b1"
+    using diff_ab subbtr_id id_set_notempty by fastforce
+  have n2: "\<not> id_set subbtr \<subseteq> id_set b3"
+    using diff_bc subbtr_id id_set_notempty by fastforce
+  have n3: "\<not> id_set subbtr \<subseteq> id_set b4"
+    using diff_bd subbtr_id id_set_notempty by fastforce
+  show ?thesis using n1 n2 n3 unfolding id_set_def
+    by (metis subset_image_iff tree.set_map)
+qed
+
+lemma diff_node3:
+  "diff_ids (Node b1 b2 b3 b4) \<Longrightarrow>
+  tree.set subbtr \<subseteq> tree.set b3 \<Longrightarrow>
+  \<not> tree.set subbtr \<subseteq> tree.set b1 \<and> \<not> tree.set subbtr \<subseteq> tree.set b2 \<and> \<not> tree.set subbtr \<subseteq> tree.set b4"
+proof-
+  assume a0: "diff_ids (Node b1 b2 b3 b4)"
+     and a1: "tree.set subbtr \<subseteq> tree.set b3"
+  have diff_ac: "(id_set b3) \<inter> (id_set b1) = {}"
+    using a0 diff_ids_leaf_node(2) by blast
+  have diff_bc: "(id_set b3) \<inter> (id_set b2) = {}"
+    using a0 diff_ids_leaf_node(2) by blast
+  have diff_cd: "(id_set b3) \<inter> (id_set b4) = {}"
+    using a0 diff_ids_leaf_node(2) by blast
+  have subbtr_id: "id_set subbtr \<subseteq> id_set b3"
+    unfolding id_set_def using a1
+    by (metis subset_image_iff tree.set_map)
+  have n1: "\<not> id_set subbtr \<subseteq> id_set b1"
+    using diff_ac subbtr_id id_set_notempty by fastforce
+  have n2: "\<not> id_set subbtr \<subseteq> id_set b2"
+    using diff_bc subbtr_id id_set_notempty by fastforce
+  have n3: "\<not> id_set subbtr \<subseteq> id_set b4"
+    using diff_cd subbtr_id id_set_notempty by fastforce
+  show ?thesis using n1 n2 n3 unfolding id_set_def
+    by (metis subset_image_iff tree.set_map)
+qed
+
+lemma diff_node4:
+  "diff_ids (Node b1 b2 b3 b4) \<Longrightarrow>
+  tree.set subbtr \<subseteq> tree.set b4 \<Longrightarrow>
+  \<not> tree.set subbtr \<subseteq> tree.set b1 \<and> \<not> tree.set subbtr \<subseteq> tree.set b2 \<and> \<not> tree.set subbtr \<subseteq> tree.set b3"
+proof-
+  assume a0: "diff_ids (Node b1 b2 b3 b4)"
+     and a1: "tree.set subbtr \<subseteq> tree.set b4"
+  have diff_ad: "(id_set b4) \<inter> (id_set b1) = {}"
+    using a0 diff_ids_leaf_node(2) by blast
+  have diff_bd: "(id_set b4) \<inter> (id_set b2) = {}"
+    using a0 diff_ids_leaf_node(2) by blast
+  have diff_cd: "(id_set b4) \<inter> (id_set b3) = {}"
+    using a0 diff_ids_leaf_node(2) by blast
+  have subbtr_id: "id_set subbtr \<subseteq> id_set b4"
+    unfolding id_set_def using a1
+    by (metis subset_image_iff tree.set_map)
+  have n1: "\<not> id_set subbtr \<subseteq> id_set b1"
+    using diff_ad subbtr_id id_set_notempty by fastforce
+  have n2: "\<not> id_set subbtr \<subseteq> id_set b2"
+    using diff_bd subbtr_id id_set_notempty by fastforce
+  have n3: "\<not> id_set subbtr \<subseteq> id_set b3"
+    using diff_cd subbtr_id id_set_notempty by fastforce
+  show ?thesis using n1 n2 n3 unfolding id_set_def
+    by (metis subset_image_iff tree.set_map)
+qed
+
+definition "diff_ids_valid bset \<equiv> 
+  (\<forall>b \<in> bset. diff_ids b) \<and> 
+  (\<forall>b1 b2. b1 \<in> bset \<and> b2 \<in> bset \<and> b1 \<noteq> b2 \<longrightarrow> id_set b1 \<inter> id_set b2 = {})"
+
+lemma same_ids_replace:
+  "diff_ids B \<Longrightarrow>
+  L b \<in> set B \<Longrightarrow>
+  b' = set_state_type b t \<Longrightarrow>
+  id_set B = id_set (replace B b b')"
+proof(induct B)
+  case (Leaf x)
+  have leaf_b: "L b = x"
+    using Leaf.prems(2) by auto
+  have leaf_b': "b' = Leaf (t, snd x)"
+    using Leaf.prems(3) leaf_b unfolding set_state_type_def Let_def by auto
+  have leaf_B': "replace (Leaf x) b b' = Leaf (t, snd x)"
+    using leaf_b leaf_b' unfolding replace_def by auto
+  then show ?case unfolding id_set_def by auto
+next
+  case (Node b1 b2 b3 b4)
+  have diff_b1: "diff_ids b1"
+    using Node.prems(1) diff_ids_leaf_node(2) by blast
+  have diff_b2: "diff_ids b2"
+    using Node.prems(1) diff_ids_leaf_node(2) by blast
+  have diff_b3: "diff_ids b3"
+    using Node.prems(1) diff_ids_leaf_node(2) by blast
+  have diff_b4: "diff_ids b4"
+    using Node.prems(1) diff_ids_leaf_node(2) by blast
+  have diff_ab: "(id_set b1) \<inter> (id_set b2) = {}"
+    using Node.prems(1) diff_ids_leaf_node(2) by blast
+  have diff_ac: "(id_set b1) \<inter> (id_set b3) = {}"
+    using Node.prems(1) diff_ids_leaf_node(2) by blast
+  have diff_ad: "(id_set b1) \<inter> (id_set b4) = {}"
+    using Node.prems(1) diff_ids_leaf_node(2) by blast
+  have diff_bc: "(id_set b2) \<inter> (id_set b3) = {}"
+    using Node.prems(1) diff_ids_leaf_node(2) by blast
+  have diff_bd: "(id_set b2) \<inter> (id_set b4) = {}"
+    using Node.prems(1) diff_ids_leaf_node(2) by blast
+  have diff_cd: "(id_set b3) \<inter> (id_set b4) = {}"
+    using Node.prems(1) diff_ids_leaf_node(2) by blast
+  {assume a0: "L b \<in> set b1"
+    have no_belong_b2: "L b \<notin> set b2"
+      using a0 diff_ab unfolding id_set_def
+      by (metis disjoint_iff_not_equal image_eqI tree.set_map)
+    have no_belong_b3: "L b \<notin> set b3"
+      using a0 diff_ac unfolding id_set_def
+      by (metis disjoint_iff_not_equal image_eqI tree.set_map)
+    have no_belong_b4: "L b \<notin> set b4"
+      using a0 diff_ad unfolding id_set_def
+      by (metis disjoint_iff_not_equal image_eqI tree.set_map)
+    have replace_re: "replace (Node b1 b2 b3 b4) b b' = Node (replace b1 b b') b2 b3 b4"
+      using a0 unfolding replace_def apply auto
+      using no_replace no_belong_b2 Node.prems(3) apply auto[1]
+      using no_replace no_belong_b3 Node.prems(3) apply auto[1]
+      using no_replace no_belong_b4 Node.prems(3) by auto
+    have same_b1': "id_set b1 = id_set (replace b1 b b')"
+      using Node.hyps(1) diff_b1 a0 Node.prems(3) by auto
+    have ?case using replace_re id_set_node same_b1' by auto
+  }
+  moreover
+  {assume a1: "L b \<in> set b2"
+    have no_belong_b1: "L b \<notin> set b1"
+      using a1 diff_ab unfolding id_set_def
+      by (metis disjoint_iff_not_equal image_eqI tree.set_map)
+    have no_belong_b3: "L b \<notin> set b3"
+      using a1 diff_bc unfolding id_set_def
+      by (metis disjoint_iff_not_equal image_eqI tree.set_map)
+    have no_belong_b4: "L b \<notin> set b4"
+      using a1 diff_bd unfolding id_set_def
+      by (metis disjoint_iff_not_equal image_eqI tree.set_map)
+    have replace_re: "replace (Node b1 b2 b3 b4) b b' = Node b1 (replace b2 b b') b3 b4"
+      using a1 unfolding replace_def apply auto
+      using no_replace no_belong_b1 Node.prems(3) apply auto[1]
+      using no_replace no_belong_b3 Node.prems(3) apply auto[1]
+      using no_replace no_belong_b4 Node.prems(3) by auto
+    have same_b2': "id_set b2 = id_set (replace b2 b b')"
+      using Node.hyps(2) diff_b2 a1 Node.prems(3) by auto
+    have ?case using replace_re id_set_node same_b2' by auto
+  }
+  moreover
+  {assume a2: "L b \<in> set b3"
+    have no_belong_b1: "L b \<notin> set b1"
+      using a2 diff_ac unfolding id_set_def
+      by (metis disjoint_iff_not_equal image_eqI tree.set_map)
+    have no_belong_b2: "L b \<notin> set b2"
+      using a2 diff_bc unfolding id_set_def
+      by (metis disjoint_iff_not_equal image_eqI tree.set_map)
+    have no_belong_b4: "L b \<notin> set b4"
+      using a2 diff_cd unfolding id_set_def
+      by (metis disjoint_iff_not_equal image_eqI tree.set_map)
+    have replace_re: "replace (Node b1 b2 b3 b4) b b' = Node b1 b2 (replace b3 b b') b4"
+      using a2 unfolding replace_def apply auto
+      using no_replace no_belong_b1 Node.prems(3) apply auto[1]
+      using no_replace no_belong_b2 Node.prems(3) apply auto[1]
+      using no_replace no_belong_b4 Node.prems(3) by auto
+    have same_b3': "id_set b3 = id_set (replace b3 b b')"
+      using Node.hyps(3) diff_b3 a2 Node.prems(3) by auto
+    have ?case using replace_re id_set_node same_b3' by auto
+  }
+  moreover
+  {assume a3: "L b \<in> set b4"
+    have no_belong_b1: "L b \<notin> set b1"
+      using a3 diff_ad unfolding id_set_def
+      by (metis disjoint_iff_not_equal image_eqI tree.set_map)
+    have no_belong_b2: "L b \<notin> set b2"
+      using a3 diff_bd unfolding id_set_def
+      by (metis disjoint_iff_not_equal image_eqI tree.set_map)
+    have no_belong_b3: "L b \<notin> set b3"
+      using a3 diff_cd unfolding id_set_def
+      by (metis disjoint_iff_not_equal image_eqI tree.set_map)
+    have replace_re: "replace (Node b1 b2 b3 b4) b b' = Node b1 b2 b3 (replace b4 b b')"
+      using a3 unfolding replace_def apply auto
+      using no_replace no_belong_b1 Node.prems(3) apply auto[1]
+      using no_replace no_belong_b2 Node.prems(3) apply auto[1]
+      using no_replace no_belong_b3 Node.prems(3) by auto
+    have same_b4': "id_set b4 = id_set (replace b4 b b')"
+      using Node.hyps(4) diff_b4 a3 Node.prems(3) by auto
+    have ?case using replace_re id_set_node same_b4' by auto
+  }
+  ultimately have ?case using Node.prems(2) by fastforce
+  then show ?case by auto
+qed
+
+lemma diff_ids_replace:
+  "diff_ids B \<Longrightarrow>
+  L b \<in> set B \<Longrightarrow>
+  b' = set_state_type b t \<Longrightarrow>
+  diff_ids (replace B b b')"
+proof(induct B)
+  case (Leaf x)
+  have leaf_b: "L b = x"
+    using Leaf.prems(2) by fastforce
+  have leaf_b': "b' = Leaf (t, snd x)"
+    using Leaf.prems(3) leaf_b unfolding set_state_type_def Let_def by auto
+  have leaf_B': "replace (Leaf x) b b' = Leaf (t, snd x)"
+    using leaf_b leaf_b' unfolding replace_def by auto
+  then show ?case using diff1 by auto
+next
+  case (Node b1 b2 b3 b4)
+  have diff_b1: "diff_ids b1"
+    using Node.prems(1) diff_ids_leaf_node(2) by blast
+  have diff_b2: "diff_ids b2"
+    using Node.prems(1) diff_ids_leaf_node(2) by blast
+  have diff_b3: "diff_ids b3"
+    using Node.prems(1) diff_ids_leaf_node(2) by blast
+  have diff_b4: "diff_ids b4"
+    using Node.prems(1) diff_ids_leaf_node(2) by blast
+  have diff_ab: "(id_set b1) \<inter> (id_set b2) = {}"
+    using Node.prems(1) diff_ids_leaf_node(2) by blast
+  have diff_ac: "(id_set b1) \<inter> (id_set b3) = {}"
+    using Node.prems(1) diff_ids_leaf_node(2) by blast
+  have diff_ad: "(id_set b1) \<inter> (id_set b4) = {}"
+    using Node.prems(1) diff_ids_leaf_node(2) by blast
+  have diff_bc: "(id_set b2) \<inter> (id_set b3) = {}"
+    using Node.prems(1) diff_ids_leaf_node(2) by blast
+  have diff_bd: "(id_set b2) \<inter> (id_set b4) = {}"
+    using Node.prems(1) diff_ids_leaf_node(2) by blast
+  have diff_cd: "(id_set b3) \<inter> (id_set b4) = {}"
+    using Node.prems(1) diff_ids_leaf_node(2) by blast
+  {assume a0: "L b \<in> set b1"
+    have no_belong_b2: "L b \<notin> set b2"
+      using a0 diff_ab unfolding id_set_def
+      by (metis disjoint_iff_not_equal image_eqI tree.set_map)
+    have no_belong_b3: "L b \<notin> set b3"
+      using a0 diff_ac unfolding id_set_def
+      by (metis disjoint_iff_not_equal image_eqI tree.set_map)
+    have no_belong_b4: "L b \<notin> set b4"
+      using a0 diff_ad unfolding id_set_def
+      by (metis disjoint_iff_not_equal image_eqI tree.set_map)
+    have replace_re: "replace (Node b1 b2 b3 b4) b b' = Node (replace b1 b b') b2 b3 b4"
+      using a0 unfolding replace_def apply auto
+      using no_replace no_belong_b2 Node.prems(3) apply auto[1]
+      using no_replace no_belong_b3 Node.prems(3) apply auto[1]
+      using no_replace no_belong_b4 Node.prems(3) by auto
+    have diff_b1': "diff_ids (replace b1 b b')"
+      using Node.hyps(1) diff_b1 a0 Node.prems(3) by auto
+    have diff_ab': "id_set (replace b1 b b') \<inter> id_set b2 = {}"
+      using same_ids_replace diff_b1 a0 Node.prems(3) diff_ab by auto
+    have diff_ac': "id_set (replace b1 b b') \<inter> id_set b3 = {}"
+      using same_ids_replace diff_b1 a0 Node.prems(3) diff_ac by auto
+    have diff_ad': "id_set (replace b1 b b') \<inter> id_set b4 = {}"
+      using same_ids_replace diff_b1 a0 Node.prems(3) diff_ad by auto
+    have ?case using replace_re diff_b1' diff_b2 diff_b3 diff_b4 diff_ab' diff_ac' diff_ad' diff_bc diff_bd diff_cd diff2 by auto
+  }
+  moreover
+  {assume a1: "L b \<in> set b2"
+    have no_belong_b1: "L b \<notin> set b1"
+      using a1 diff_ab unfolding id_set_def
+      by (metis disjoint_iff_not_equal image_eqI tree.set_map)
+    have no_belong_b3: "L b \<notin> set b3"
+      using a1 diff_bc unfolding id_set_def
+      by (metis disjoint_iff_not_equal image_eqI tree.set_map)
+    have no_belong_b4: "L b \<notin> set b4"
+      using a1 diff_bd unfolding id_set_def
+      by (metis disjoint_iff_not_equal image_eqI tree.set_map)
+    have replace_re: "replace (Node b1 b2 b3 b4) b b' = Node b1 (replace b2 b b') b3 b4"
+      using a1 unfolding replace_def apply auto
+      using no_replace no_belong_b1 Node.prems(3) apply auto[1]
+      using no_replace no_belong_b3 Node.prems(3) apply auto[1]
+      using no_replace no_belong_b4 Node.prems(3) by auto
+    have diff_b2': "diff_ids (replace b2 b b')"
+      using Node.hyps(2) diff_b2 a1 Node.prems(3) by auto
+    have diff_ab': "id_set (replace b2 b b') \<inter> id_set b1 = {}"
+      using same_ids_replace diff_b2 a1 Node.prems(3) diff_ab by auto
+    have diff_bc': "id_set (replace b2 b b') \<inter> id_set b3 = {}"
+      using same_ids_replace diff_b2 a1 Node.prems(3) diff_bc by auto
+    have diff_bd': "id_set (replace b2 b b') \<inter> id_set b4 = {}"
+      using same_ids_replace diff_b2 a1 Node.prems(3) diff_bd by auto
+    have ?case using replace_re diff_b1 diff_b2' diff_b3 diff_b4 diff_ab' diff_ac diff_ad diff_bc' diff_bd' diff_cd diff2 by (simp add: inf_commute) 
+  }
+  moreover
+  {assume a2: "L b \<in> set b3"
+    have no_belong_b1: "L b \<notin> set b1"
+      using a2 diff_ac unfolding id_set_def
+      by (metis disjoint_iff_not_equal image_eqI tree.set_map)
+    have no_belong_b2: "L b \<notin> set b2"
+      using a2 diff_bc unfolding id_set_def
+      by (metis disjoint_iff_not_equal image_eqI tree.set_map)
+    have no_belong_b4: "L b \<notin> set b4"
+      using a2 diff_cd unfolding id_set_def
+      by (metis disjoint_iff_not_equal image_eqI tree.set_map)
+    have replace_re: "replace (Node b1 b2 b3 b4) b b' = Node b1 b2 (replace b3 b b') b4"
+      using a2 unfolding replace_def apply auto
+      using no_replace no_belong_b1 Node.prems(3) apply auto[1]
+      using no_replace no_belong_b2 Node.prems(3) apply auto[1]
+      using no_replace no_belong_b4 Node.prems(3) by auto
+    have diff_b3': "diff_ids (replace b3 b b')"
+      using Node.hyps(3) diff_b3 a2 Node.prems(3) by auto
+    have diff_ac': "id_set (replace b3 b b') \<inter> id_set b1 = {}"
+      using same_ids_replace diff_b3 a2 Node.prems(3) diff_ac by auto
+    have diff_bc': "id_set (replace b3 b b') \<inter> id_set b2 = {}"
+      using same_ids_replace diff_b3 a2 Node.prems(3) diff_bc by auto
+    have diff_cd': "id_set (replace b3 b b') \<inter> id_set b4 = {}"
+      using same_ids_replace diff_b3 a2 Node.prems(3) diff_cd by auto
+    have ?case using replace_re diff_b1 diff_b2 diff_b3' diff_b4 diff_ab diff_ac' diff_ad diff_bc' diff_bd diff_cd' diff2 by (simp add: inf_commute) 
+  }
+  moreover
+  {assume a3: "L b \<in> set b4"
+    have no_belong_b1: "L b \<notin> set b1"
+      using a3 diff_ad unfolding id_set_def
+      by (metis disjoint_iff_not_equal image_eqI tree.set_map)
+    have no_belong_b2: "L b \<notin> set b2"
+      using a3 diff_bd unfolding id_set_def
+      by (metis disjoint_iff_not_equal image_eqI tree.set_map)
+    have no_belong_b3: "L b \<notin> set b3"
+      using a3 diff_cd unfolding id_set_def
+      by (metis disjoint_iff_not_equal image_eqI tree.set_map)
+    have replace_re: "replace (Node b1 b2 b3 b4) b b' = Node b1 b2 b3 (replace b4 b b')"
+      using a3 unfolding replace_def apply auto
+      using no_replace no_belong_b1 Node.prems(3) apply auto[1]
+      using no_replace no_belong_b2 Node.prems(3) apply auto[1]
+      using no_replace no_belong_b3 Node.prems(3) by auto
+    have diff_b4': "diff_ids (replace b4 b b')"
+      using Node.hyps(4) diff_b4 a3 Node.prems(3) by auto
+    have diff_ad': "id_set (replace b4 b b') \<inter> id_set b1 = {}"
+      using same_ids_replace diff_b4 a3 Node.prems(3) diff_ad by auto
+    have diff_bd': "id_set (replace b4 b b') \<inter> id_set b2 = {}"
+      using same_ids_replace diff_b4 a3 Node.prems(3) diff_bd by auto
+    have diff_cd': "id_set (replace b4 b b') \<inter> id_set b3 = {}"
+      using same_ids_replace diff_b4 a3 Node.prems(3) diff_cd by auto
+    have ?case using replace_re diff_b1 diff_b2 diff_b3 diff_b4' diff_ab diff_ac diff_ad' diff_bc diff_bd' diff_cd' diff2 by (simp add: inf_commute)
+  }
+  ultimately have ?case using Node.prems(2) by fastforce
+  then show ?case by auto
+qed
+
+
 
 
 definition getnewid :: "ID set \<Rightarrow> (ID \<times> ID \<times> ID \<times> ID \<times> ID set)"
@@ -472,7 +1051,8 @@ lemma elem_in_diff_set:"card s = n \<Longrightarrow>
        card s' <n \<Longrightarrow> \<exists>x.  x\<in> s - s'"
   by (meson all_not_in_conv diff_set_not_empty)
 
-lemma assumes a0:"finite ids"      
+lemma divide_not_empty:
+  assumes a0:"finite ids"      
   shows "divide ids \<noteq> {}"
 proof-
    obtain s where s:"((card s = 4 \<and> s \<inter> ids = {}))"
@@ -491,7 +1071,8 @@ proof-
     using s x1_in_s x2_in_s x3_in_s x4_in_s apply auto   by metis    
 qed  
 
-lemma divide_dest1:assumes a0:"finite ids" 
+
+lemma divide_dest1:
   shows "\<forall>node\<in> divide ids. snd ` set node \<inter> ids = {}"
 proof-   
   let ?ids = "{s. (card s = 4 \<and> s \<inter> ids = {})}" 
@@ -505,9 +1086,13 @@ proof-
     then have "snd ` set node \<inter> ids = {}"
       by auto
   } thus ?thesis by auto
-qed
+qed      
 
-lemma divide_dest2:assumes a0:"finite ids" 
+lemma divide_dest1a:
+  shows "n\<in> divide ids \<Longrightarrow> snd ` set n  \<inter> ids = {}"
+  using divide_dest1 by auto
+
+lemma divide_dest2: 
   shows "\<forall>node\<in> divide ids. card (set node) = 4"
 proof-   
   let ?ids = "{s. (card s = 4 \<and> s \<inter> ids = {})}" 
@@ -523,25 +1108,48 @@ proof-
   } thus ?thesis by auto
 qed
 
-lemma divide_dest3:assumes a0:"finite ids" and 
-   a2: "(Node n1 n2 n3 n4) \<in> divide ids"
+lemma divide_dest3:assumes  
+   a0: "(Node n1 n2 n3 n4) \<in> divide ids"
  shows "leaf n1 \<and> leaf n2 \<and> leaf n3 \<and> leaf n4 \<and>
         snd (L n1) \<noteq> snd (L n2) \<and> snd (L n1) \<noteq> snd (L n3) \<and> snd (L n1) \<noteq> snd (L n4) \<and> 
-        snd (L n2) \<noteq> snd (L n1) \<and> snd (L n2) \<noteq> snd (L n3) \<and> snd (L n3)\<noteq> snd (L n4)"
+        snd (L n2) \<noteq> snd (L n3) \<and> snd (L n2) \<noteq> snd (L n4) \<and> snd (L n3)\<noteq> snd (L n4)"
 proof-   
   let ?ids = "{s. (card s = 4 \<and> s \<inter> ids = {})}" 
   let ?node = "(Node n1 n2 n3 n4)"
    obtain s x1 x2 x3 x4 where 
        spec:"s \<in> ?ids \<and> x1 \<in> s \<and> x2 \<in> s - {x1} \<and> x3 \<in> s - {x1,x2} \<and> x4 \<in> s -{x1,x2,x3} \<and>
         ?node = (Node (Leaf (ALLOC, x1)) (Leaf (FREE, x2)) (Leaf (FREE, x3)) (Leaf (FREE, x4)))"
-      using a2 unfolding divide_def by auto    
+      using a0 unfolding divide_def by auto    
     then have "leaf n1 \<and> leaf n2 \<and> leaf n3 \<and> leaf n4 \<and>
         snd (L n1) \<noteq> snd (L n2) \<and> snd (L n1) \<noteq> snd (L n3) \<and> snd (L n1) \<noteq> snd (L n4) \<and> 
-        snd (L n2) \<noteq> snd (L n1) \<and> snd (L n2) \<noteq> snd (L n3) \<and> snd (L n3)\<noteq> snd (L n4)"
+        snd (L n2) \<noteq> snd (L n3) \<and> snd (L n2) \<noteq> snd (L n4) \<and> snd (L n3)\<noteq> snd (L n4)"
       by auto
   thus ?thesis by auto
 qed
 
+lemma divide_dest3a:assumes  
+   a0: "(Node n1 n2 n3 n4) \<in> divide ids"
+ shows "\<exists>n1a n2a n3a n4a. n1 = Leaf n1a \<and> n2 = Leaf n2a \<and> n3= Leaf n3a \<and> n4 = Leaf n4a \<and>
+        snd n1a \<noteq> snd n2a \<and> snd n1a \<noteq> snd n3a \<and> snd n1a \<noteq> snd n4a \<and> 
+        snd n2a \<noteq> snd n3a \<and> snd n2a \<noteq> snd n4a \<and> snd n3a \<noteq> snd n4a"
+  using divide_dest3[OF a0]
+  by (metis (no_types) tree.collapse(1)) 
+
+lemma divide_dest3b:assumes  
+   a0: "(Node n1 n2 n3 n4) \<in> divide ids"
+ shows "id_set n1 \<inter> id_set n2 = {} \<and> id_set n1 \<inter> id_set n3 = {} \<and> id_set n1 \<inter> id_set n4 = {} \<and>
+        id_set n2 \<inter> id_set n3 = {} \<and> id_set n2 \<inter> id_set n4 = {} \<and> id_set n3 \<inter> id_set n4 = {}"
+  using divide_dest3a[OF a0] unfolding id_set_def
+  by force
+   
+
+lemma divide_dest4:
+  shows "\<forall>n\<in> divide ids. node n"
+  unfolding divide_def by auto
+
+lemma divide_dest4a:
+  shows "n\<in> divide ids \<Longrightarrow> \<exists>n1 n2 n3 n4. n = Node n1 n2 n3 n4"
+  unfolding divide_def by auto
    
 (* definition divide :: "Block \<Rightarrow> ID set \<Rightarrow> (Block \<times> ID set)"
   where "divide bl ids \<equiv>
@@ -595,8 +1203,8 @@ proof-
   then show ?thesis using obtain_divide by auto
 qed
 *)
-definition getnewid2 :: "Block set \<Rightarrow> ID"
-  where "getnewid2 bs \<equiv> SOME p. p \<notin> (\<Union>b\<in>bs. (snd ` set b))"
+definition getnewid2 :: "ID set \<Rightarrow> ID"
+  where "getnewid2 ids \<equiv> SOME p. p \<notin> ids"
 
   
 lemma fresh_elem:"\<not> (finite (UNIV::'b set)) \<Longrightarrow> finite (bs::('a \<times> 'b) tree set) \<Longrightarrow> 
@@ -604,18 +1212,32 @@ lemma fresh_elem:"\<not> (finite (UNIV::'b set)) \<Longrightarrow> finite (bs::(
   using ex_new_if_finite finite_ids_set_set
   by blast 
 
-lemma newid_in_getnewid2: "getnewid2 bs \<in> (\<Union>b\<in>bs. (snd ` set b)) \<union> {(getnewid2 bs)}"
+lemma fresh_elem1:"\<not> (finite (UNIV::'b set)) \<Longrightarrow> finite (ids::'b set) \<Longrightarrow> 
+                    \<exists>p . p \<notin> ids"
+  using ex_new_if_finite finite_ids_set_set
+  by blast 
+
+
+lemma newid_in_getnewid2: "getnewid2 ids \<in> ids \<union> {(getnewid2 ids)}"
   unfolding getnewid2_def Let_def by auto
 
-lemma getnewid2_anot:
-  "finite bs \<Longrightarrow> bs\<noteq>{} \<Longrightarrow>
+(* lemma getnewid2_anot:
+  "finite ids \<Longrightarrow> bs\<noteq>{} \<Longrightarrow>
   xa = (getnewid2 bs) \<Longrightarrow>
   xa \<notin> (\<Union>b\<in>bs. (snd ` set b))"
   unfolding getnewid2_def Let_def
   using fresh_elem
+  by (metis infinite_UNIV_nat some_eq_ex) *)
+
+lemma getnewid2_anot:
+  "finite ids \<Longrightarrow> 
+  xa = (getnewid2 ids) \<Longrightarrow>
+  xa \<notin> ids"
+  unfolding getnewid2_def Let_def
+  using fresh_elem1
   by (metis infinite_UNIV_nat some_eq_ex)
 
-definition combine :: "Block \<Rightarrow> Block set \<Rightarrow> Block"
+definition combine :: "Block \<Rightarrow> ID set \<Rightarrow> Block"
   where "combine b bs \<equiv> (if (\<exists>a1 a2 a3 a4. b = Node (Leaf (FREE, a1)) (Leaf (FREE, a2)) (Leaf (FREE, a3)) (Leaf (FREE, a4))) then
                               (Leaf (FREE, getnewid2 bs))
                            else b)"
@@ -691,69 +1313,142 @@ qed
 
 subsection \<open>def of sub core function\<close>
 (*------------------------------------------------------------------------------------------------*)
-definition set_state_type :: "Block \<Rightarrow> block_state_type \<Rightarrow> Block"
-  where "set_state_type bl t \<equiv> (let b = (L bl) in Leaf (t, snd b))"
 
-
-fun split :: "Block \<Rightarrow> nat set \<Rightarrow> nat \<Rightarrow> Block"
+fun split :: "Block \<Rightarrow> ID set \<Rightarrow> nat \<Rightarrow> Block"
   where "split b ids lv = (if lv = 0 then b
                           else
                             let  node = SOME l. l \<in> divide ids;                                
                                 c1 = split (LL node) (ids \<union> (snd ` (set node))) (lv - 1) in
                                 Node c1 (LR node) (RL node) (RR node))"
 
-lemma split_induct:
-  "lv > 0 \<Longrightarrow>
-  Node (Leaf ll) (Leaf lr) (Leaf rl) (Leaf rr) \<in> (divide bs)  \<Longrightarrow>  
-  (split b bs lv) = Node ((split (Leaf ll) bs (lv - 1))) (Leaf lr) (Leaf rl) (Leaf rr)"
-  using split.simps unfolding Let_def sorry
-  by (metis fst_conv less_not_refl3 tree.sel(2) tree.sel(3) tree.sel(4) tree.sel(5))
+lemma divide_1:"finite ids \<Longrightarrow> (split b ids 1) = (SOME l. l \<in> divide ids)"
+  using split.simps  apply auto unfolding Let_def using divide_not_empty
+  by (metis (full_types) divide_dest4 some_in_eq tree.collapse(2))
 
-fun replace_leaf :: "Block \<Rightarrow> Block \<Rightarrow> Block \<Rightarrow> Block"
-  where "replace_leaf (Leaf x) y st = (if (x = (L y)) then st else (Leaf x))" |
-        "replace_leaf (Node n1 n2 n3 n4) y st = Node (replace_leaf n1 y st)
-                                                     (replace_leaf n2 y st)
-                                                     (replace_leaf n3 y st)
-                                                     (replace_leaf n4 y st)"
-lemma no_replace:
-  "L b \<notin> set blo \<Longrightarrow>
-  b' = set_state_type b t \<Longrightarrow>
-  tree_map (\<lambda>b1. if b1 = L b then L b' else b1) blo = blo"
-  by (smt tree.map_cong0 tree.map_ident)
+lemma split_1_nodes_not_ids:"finite ids \<Longrightarrow>  
+       (snd ` set (split b ids 1)) \<inter> ids = {}"
+  using divide_1
+  by (simp add: divide_dest1 divide_not_empty some_in_eq) 
 
-lemma no_replace_leaf:
-  "(L b) \<notin> set B \<Longrightarrow>
-  replace_leaf B b subbtr = B"
-  apply(induct B)
+
+lemma dest_set:
+  "snd ` (tree.set (Node n1 n2 n3 n4)) = snd ` (set n1) \<union> snd ` (set n2) \<union> snd ` (set n3) \<union> snd ` (set n4)"
   by auto
 
-lemma replace_leaf_belong:
-  "(L b) \<in> set B \<Longrightarrow>
-  (L l) \<in> set subbtr \<Longrightarrow>
-  (L l) \<in> set (replace_leaf B b subbtr)"
-  apply(induct B)
-  by auto
+lemma split_nodes_not_ids:"finite ids \<Longrightarrow> lv > 0  \<Longrightarrow> 
+       (snd ` set (split b ids lv)) \<inter> ids = {}"
+proof(induct lv arbitrary: ids b)
+  case 0
+  then show ?case by auto
+next
+  case Suc0:(Suc lv)
+  then show ?case 
+  proof(cases lv)
+    case 0
+    then show ?thesis using split_1_nodes_not_ids Suc0 by auto
+  next
+    let ?l = "SOME l. l \<in> Memory_Allocation_Model.divide ids"
+    case (Suc nat) 
+    have "Suc lv \<noteq> 0" using Suc by auto
+    then have split_simp:"split b ids (Suc lv) = Node (split (LL ?l) (ids \<union> snd ` tree.set ?l) lv) (LR ?l) (RL ?l) (RR ?l)"
+      using split.simps Suc unfolding Let_def
+      by (metis diff_Suc_1) 
+    obtain l where "divide ids \<noteq>{} \<and> (\<forall>l\<in>(divide ids). (snd ` set l) \<inter> ids ={} \<and> (card (set l) = 4))"
+      by (simp add: Suc0.prems(1) divide_dest1  divide_dest2 divide_not_empty)
+    then have "(snd ` set ?l) \<inter> ids ={} \<and> (card (set ?l) = 4)"
+      by (simp add: some_in_eq) 
+    moreover have "(snd `  set (split (LL ?l) (ids \<union> snd ` tree.set ?l) lv)) \<inter> (ids \<union> snd ` tree.set ?l) = {}"
+      using Suc Suc0(1,2)
+      by (simp add: finite_ids_set)            
+    ultimately show ?thesis using Suc split_simp unfolding Let_def apply auto
+      by (metis (no_types, lifting) IntI One_nat_def Suc0.prems(1) 
+                empty_iff image_eqI n_not_Suc_n snd_conv split.simps split_1_nodes_not_ids 
+                tree.disc(4) tree.sel(3,4,5) tree.set_sel(3,4,5))+
+  qed
+qed
 
-lemma replace_subbtr_belong:
-  "(L b) \<in> set B \<Longrightarrow>
-  tree.set subbtr \<subseteq> tree.set (replace_leaf B b subbtr)"
-  apply(induct B)
-  by auto
+lemma diff_ids_divide: 
+  "finite ids \<Longrightarrow> l\<in>Memory_Allocation_Model.divide ids \<Longrightarrow> diff_ids l"
+  apply (frule divide_dest4a)  
+  using diff2 unfolding id_set_def
+  by (auto simp: diff1  dest: divide_dest4a divide_dest3b divide_dest3a)
+  
+lemma split_nodes_diff_ids1:
+      "finite ids \<Longrightarrow> 
+       diff_ids (split b ids 1)"
+  using  diff_ids_divide divide_not_empty some_in_eq
+  by (metis divide_1)
+                        
+lemma split_nodes_diff_idsn:
+      "diff_ids b  \<Longrightarrow> finite ids \<Longrightarrow> lv > 0 \<Longrightarrow>
+       diff_ids (split b ids lv)"
+proof(induct lv arbitrary: ids b)
+  case 0
+  then show ?case by auto
+next
+  case Suc0:(Suc lv)
+  then show ?case 
+  proof(cases lv)
+    case 0
+    then show ?thesis  using split_nodes_diff_ids1 Suc0  by auto
+  next
+   let ?l = "SOME l. l \<in> Memory_Allocation_Model.divide ids"
+    case (Suc nat) 
+    have "Suc lv \<noteq> 0" using Suc by auto
+    then have split_simp:"split b ids (Suc lv) = Node (split (LL ?l) (ids \<union> snd ` tree.set ?l) lv) (LR ?l) (RL ?l) (RR ?l)"
+      using split.simps Suc  unfolding Let_def
+      by (metis diff_Suc_1)         
+    have  "snd ` (set (split (LL ?l) (ids \<union> snd ` tree.set ?l) lv)) \<inter> snd ` (set (LR ?l)) = {} \<and>
+           snd ` (set (split (LL ?l) (ids \<union> snd ` tree.set ?l) lv)) \<inter> snd ` (set (RL ?l)) = {} \<and>
+           snd ` (set (split (LL ?l) (ids \<union> snd ` tree.set ?l) lv)) \<inter> snd ` (set (RR ?l)) = {}"
+    proof-      
+      have "finite (ids \<union> snd ` tree.set ?l)" using Suc0(3)
+        using finite_ids_set by blast
+      moreover have "0< lv" using Suc0(4)
+        by (simp add: Suc)
+      ultimately have "snd ` (set (split (LL ?l) (ids \<union> snd ` tree.set ?l) lv)) \<inter> (ids \<union> snd ` tree.set ?l) = {}"
+        using split_nodes_not_ids by auto
+      moreover have "snd ` (set (LR ?l)) \<subseteq> snd ` (tree.set ?l) \<and> snd ` (set (RL ?l)) \<subseteq> snd ` (tree.set ?l) \<and> 
+                   snd ` (set (RR ?l)) \<subseteq> snd ` (tree.set ?l)"
+        by (metis Suc0.prems(2) divide_dest4 divide_not_empty image_mono some_in_eq subsetI 
+            tree.set_sel(3,4,5))
+      ultimately show ?thesis
+        by (simp add: disjoint_iff_not_equal subset_eq) 
+    qed
+    moreover have "snd ` tree.set (LR ?l) \<inter> snd ` tree.set (RL ?l) = {} \<and> 
+                   snd ` tree.set (LR ?l) \<inter> snd ` tree.set (RR ?l) = {} \<and>
+                   snd ` tree.set (RL ?l) \<inter> snd ` tree.set (RR ?l) = {}"
+      by (metis Suc0.prems(2) diff_ids_divide diff_ids_leaf_node(2) 
+                divide_dest4 divide_not_empty id_set_def some_in_eq tree.collapse(2)) 
+    moreover have "diff_ids (LR ?l) \<and> diff_ids (RL ?l) \<and> diff_ids (RR ?l)" using Suc0
+      by (metis  diff1 divide_dest3 divide_dest4 divide_not_empty  
+           some_in_eq tree.collapse(1) tree.collapse(2))
+    moreover have "diff_ids (split (LL ?l) (ids \<union> snd ` tree.set ?l) lv)" using Suc0
+      by (metis Suc diff1 divide_dest3 divide_dest4 divide_not_empty finite_Un 
+          finite_ids_set some_in_eq tree.collapse(1) tree.collapse(2) zero_less_Suc)      
+    ultimately show ?thesis using diff2 split_nodes_not_ids divide_dest3b divide_dest3a  
+      by (simp only: split_simp id_set_def )      
+  qed 
+qed
+  
+lemma split_node_diff_ids2:
+      "diff_ids b  \<Longrightarrow> lv = 0 \<Longrightarrow>
+       diff_ids (split b ids lv)"
+  unfolding split_def by auto
 
-fun merge :: "Block \<Rightarrow> Block set \<Rightarrow> Block"
-  where "merge (Leaf v) bs = (Leaf v)" |
-        "merge (Node ll lr rl rr) bs =
-                (if (\<exists>xa xb xc xd. (Node ll lr rl rr) = Node (Leaf (FREE, xa))
-                                                             (Leaf (FREE, xb))
-                                                             (Leaf (FREE, xc))
-                                                             (Leaf (FREE, xd)))
-                 then combine (Node ll lr rl rr) bs
-                 else
-                    let m1 = merge ll bs;
-                        m2 = merge lr bs;
-                        m3 = merge rl bs;
-                        m4 = merge rr bs in
-                    combine (Node m1 m2 m3 m3) bs)"
+lemma split_nodes_diff_ids:
+      "diff_ids b  \<Longrightarrow> finite ids \<Longrightarrow> 
+       diff_ids (split b ids lv)"
+  using split_nodes_diff_idsn split_node_diff_ids2 by auto
+
+fun merge :: "Block \<Rightarrow> ID set \<Rightarrow> Block"
+  where "merge (Leaf v) ids = (Leaf v)" |
+        "merge (Node ll lr rl rr) ids =                
+                    (let m1 = merge ll ids;
+                        m2 = merge lr (ids \<union> snd ` (set m1));
+                        m3 = merge rl (ids \<union> (snd ` (set m1)) \<union> (snd ` (set m2))) ;
+                        m4 = merge rr (ids \<union> (snd ` (set m1)) \<union> (snd ` (set m2)) \<union> (snd ` (set m3))) in
+                    combine (Node m1 m2 m3 m3) (ids \<union> (snd ` (set m1)) \<union> (snd ` (set m2)) \<union> (snd ` (set m3)) \<union> (snd ` (set m4))))"
 
 definition alloc1 :: "Block set \<Rightarrow> nat \<Rightarrow>  (Block set \<times>  bool)"
   where "alloc1 bset lv  \<equiv> (let blo = (SOME b. b \<in> bset \<and> freesets_level b lv \<noteq> {});
@@ -783,7 +1478,7 @@ definition free :: "Block set \<Rightarrow> Block \<Rightarrow>(Block set \<time
             else
                 let btree = (THE t. t \<in> bset \<and> (L b) \<in> set t);
                     freeblo = replace btree b (set_state_type b FREE) in
-                ((bset - {btree}) \<union> {merge freeblo bset}, True)
+                ((bset - {btree}) \<union> {merge freeblo (\<Union>b\<in>bset. (snd ` set b))}, True)
          else
             (bset, False)"
 
